theories/Spilling/RepairSpillSound.v
@@ -1,4 +1,4 @@
-Require Import RepairSpill RegLive.
+Require Import RepairSpill RegLive ExpVarsBounded.
 Require Import SpillSound Annotation Liveness.Liveness RenamedApart.
 Require Import List Map IL.
 Require Import Take TakeSet.
@@ -8,6 +8,22 @@ Set Implicit Arguments.
 (** * Soundness of repair_spill *)
 
 
+Lemma set_union_disjunctify (X:Type) `{OrderedType X} (s t : ⦃X⦄) :
+  s ∪ t [=] (s \ t) ∪ (s ∩ t) ∪ (t \ s)
+.
+Proof.
+  cset_tac.
+Qed.
+
+Lemma cardinal_union_split (X:Type) `{OrderedType X} (s t : ⦃X⦄) :
+  cardinal (s ∪ t) = cardinal (s \ t) + cardinal (s ∩ t) + cardinal (t \ s)
+.
+Proof.
+  rewrite <-union_cardinal; [|cset_tac]. setoid_rewrite union_comm at 2. rewrite <-set_decomp.
+  rewrite <-union_cardinal; [|cset_tac]. apply Equal_cardinal. cset_tac.
+Qed.
+
+
 Lemma repair_spill_sound k ZL Λ R M s rlv lv sl (*ra*)
   : live_sound Imperative ZL (merge ⊝ Λ) s lv
     -> annotation s sl
@@ -15,21 +31,25 @@ Lemma repair_spill_sound k ZL Λ R M s rlv lv sl (*ra*)
 (*    -> renamedApart s ra
     -> R ∪ M [=] fst (getAnn ra)*)
     -> getAnn lv ⊆ R ∪ M
+    -> exp_vars_bounded k s
     -> spill_sound k ZL Λ (R,M) s (repair_spill k ZL Λ R M s rlv lv sl)
 .
 Proof.
-  intros lvSnd anno_sl anno_rlv lv_RM (*rena RM_ra*).
-  general induction lvSnd; invc anno_sl; invc anno_rlv; (*invc rena;*) cbn.
+  intros lvSnd anno_sl anno_rlv lv_RM expB (*rena RM_ra*).
+  general induction lvSnd; invc anno_sl; invc anno_rlv; invc expB; (*invc rena;*) cbn.
   - destruct a,p. rename s0 into Sp. rename s1 into L. rename a0 into Rlv.
-    set (L' := set_take_prefer k (L ∩ (Sp ∩ R ∪ M)) (Exp.freeVars e \ R)) in *.
-    set (K' := set_take_least_avoid (cardinal (R ∪ L') - k) (R \ (Exp.freeVars e ∪ L')) Rlv) in *.
-    set (Kx' := set_take_least_avoid (cardinal {x; R \ K' ∪ L'} - k) R Rlv) in *.
+    set (L' := set_take_prefer (k - cardinal (Exp.freeVars e ∩ R \ L))
+                               (L ∩ (Sp ∩ R ∪ M)) (Exp.freeVars e \ R)) in *.
+    set (K' := set_take_least_avoid ((cardinal R + cardinal L') - k)
+                                    ((R \ Exp.freeVars e) ∪ (R ∩ L')) Rlv) in *.
+    set (Kx' := set_take_least_avoid (cardinal {x; R \ K' ∪ L'} - k) (R \ K' ∪ L') Rlv) in *.
     set (Sp':= (getAnn al ∩ (K' ∪ Kx') \ M ∪ (Sp ∩ R))) in *.
     assert (Sp ∩ R ⊆ Sp') as Spincl.
     { subst Sp'. clear; cset_tac. }
     econstructor; eauto.
     + subst Sp'. apply incl_minus_incl_union in H0. rewrite H0.
-      subst Kx'. rewrite set_take_least_avoid_incl. subst K'. rewrite set_take_least_avoid_incl.
+      subst Kx'. rewrite set_take_least_avoid_incl. subst K'.
+      setoid_rewrite set_take_least_avoid_incl at 1.
       clear; cset_tac.
     + subst L'. rewrite set_take_prefer_incl. rewrite Spincl.
       cbn in *. apply Exp.freeVars_live in H. rewrite H. clear - lv_RM. cset_tac.
@@ -42,7 +62,39 @@ Proof.
       setoid_rewrite set_decomp with (t:=(K' ∪ Kx')) at 1.
       apply union_incl_split; [|cset_tac]. setoid_rewrite <-incl_right at 2.
       setoid_rewrite set_decomp with (t:=M) at 1; cset_tac.
-    + eapply Exp.freeVars_live in H. rewrite H. subst L'. 
+    + subst L'. cbn in *. 
+      subst K'. rewrite set_take_least_avoid_incl. rewrite <-set_take_prefer_card_incl.
+      * rewrite <-minus_union. clear; cset_tac.
+      * apply Nat.le_add_le_sub_l. rewrite <-union_cardinal; [|clear;cset_tac].
+        rewrite <-set_decomp. eauto.
+    + assert (K' ⊆ R) as KReq.
+      { subst K'. rewrite set_take_least_avoid_incl. clear; cset_tac. }
+      assert (disj (R \ K') L') as RKLdisj.
+      { subst K' L'.
+      setoid_rewrite set_decomp with (t:=R) at 5. rewrite <-union_assoc.
+      rewrite union_cardinal; [|clear;cset_tac].
+      setoid_rewrite cardinal_difference'.
+      setoid_rewrite set_take_least_avoid_size at 2; eauto.  
+      rewrite cardinal_union_split.
+      assert (forall s t u : ⦃var⦄, s \ t ∩ u [=] (s ∩ u) \ t) as seteq by (clear;intros;cset_tac).
+      rewrite seteq. setoid_rewrite cardinal_difference' at 2.
+
+      
+                                                                     
+                                                                     
+      subst K'. rewrite minus_union, minus_minus.
+      rewrite meet_in_left. rewrite union_cardinal_inter. subst L'.
+      apply <-Nat.le_sub_le_add_r. setoid_rewrite set_take_prefer_size at 1.
+      assert (cardinal R <= k) as cheat by admit.
+      rewrite cheat.
+      enough ((k - cardinal (Exp.freeVars e ∩ R))
+                             <= cardinal
+                                 (R ∩ set_take_prefer (k - cardinal (Exp.freeVars e ∩ R))
+                                    (L ∩ (Sp ∩ R ∪ M)) (Exp.freeVars e \ R))) by omega.
+      rewrite Nat.le_sub_le_add_r.
+      rewrite <-set_take_prefer_card_incl.
+      * 
+      setoid_rewrite set_take_prefer_incl at 2.
       cset_tac.
       subst Kx'. rewrite set_take_least_avoid_incl. subst K'. rewrite set_take_least_avoid_incl.
       cbn in *. subst Sp'. setoid_rewrite set_take_least_avoid_incl at 1.
